src/SDK/Serialize.dfy
@@ -101,10 +101,10 @@ module Serialize {
     var totalWritten := 0;
 
     // Key Value Pairs Length (number of bytes of total AAD)
-    var aadLength :- ComputeAADLength(kvPairs);
-    var len :- wr.WriteUInt16(aadLength);
+    var kvPairsLength :- ComputeKVPairsLength(kvPairs);
+    var len :- wr.WriteUInt16(kvPairsLength);
     totalWritten := totalWritten + len;
-    if aadLength == 0 {
+    if kvPairsLength == 0 {
       return Success(totalWritten);
     }
 
@@ -117,10 +117,10 @@ module Serialize {
       invariant j <= n == |kvPairs|
       invariant wr.data ==
         old(wr.data) +
-        UInt16ToSeq(aadLength) +
+        UInt16ToSeq(kvPairsLength) +
         UInt16ToSeq(n as uint16) +
-        Msg.KVPairsToSeq(kvPairs, 0, j)
-      invariant totalWritten == 4 + |Msg.KVPairsToSeq(kvPairs, 0, j)|
+        Msg.KVPairEntriesToSeq(kvPairs, 0, j)
+      invariant totalWritten == 4 + |Msg.KVPairEntriesToSeq(kvPairs, 0, j)|
     {
       len :- wr.WriteUInt16(|kvPairs[j].0| as uint16);
       totalWritten := totalWritten + len;
@@ -140,12 +140,12 @@ module Serialize {
     return Success(totalWritten);
   }
 
-  method ComputeAADLength(kvPairs: Materials.EncryptionContext) returns (res: Result<uint16>)
+  method ComputeKVPairsLength(kvPairs: Materials.EncryptionContext) returns (res: Result<uint16>)
     requires |kvPairs| < UINT16_LIMIT
     requires forall i :: 0 <= i < |kvPairs| ==> Msg.ValidKVPair(kvPairs[i])
     ensures match res
-      case Success(len) => len as int == Msg.AADLength(kvPairs)
-      case Failure(_) => UINT16_LIMIT <= Msg.AADLength(kvPairs)
+      case Success(len) => len as int == Msg.KVPairsLength(kvPairs)
+      case Failure(_) => UINT16_LIMIT <= Msg.KVPairsLength(kvPairs)
   {
     var n: int32 := |kvPairs| as int32;
     if n == 0 {
@@ -155,11 +155,11 @@ module Serialize {
       var i: int32 := 0;
       while i < n
         invariant i <= n
-        invariant 2 + Msg.KVPairsLength(kvPairs, 0, i as int) == len as int < UINT16_LIMIT
+        invariant 2 + Msg.KVPairEntriesLength(kvPairs, 0, i as int) == len as int < UINT16_LIMIT
       {
         var kvPair := kvPairs[i];
         len := len + 4 + |kvPair.0| as int32 + |kvPair.1| as int32;
-        Msg.KVPairsLengthSplit(kvPairs, 0, i as int + 1, n as int);
+        Msg.KVPairEntriesLengthSplit(kvPairs, 0, i as int + 1, n as int);
         if limit <= len {
           return Failure("The number of bytes in encryption context exceeds the allowed maximum");
         }
