test/SDK/Client.dfy
@@ -31,15 +31,15 @@ module {:extern "TestClient"} TestClient {
     var keyA, valA := UTF8.Encode("keyA").value, UTF8.Encode("valA").value;
     var encryptionContext := [(keyA, valA)];
     assert Msg.ValidAAD(encryptionContext) by {
-      // To proving ValidAAD, we need to reveal the definition of ValidAAD:
+      // To prove ValidAAD, we need to reveal the definition of ValidAAD:
       reveal Msg.ValidAAD();
-      // We also need to help the verifier with proving the AADLength is small:
+      // We also need to help the verifier with proving the KVPairsLength is small:
       calc {
-        Msg.AADLength(encryptionContext);
-        2 + Msg.KVPairsLength(encryptionContext, 0, 1);
+        Msg.KVPairsLength(encryptionContext);
+        2 + Msg.KVPairEntriesLength(encryptionContext, 0, 1);
         2 + 2 + |keyA| + 2 + |valA|;
       }
-      assert Msg.AADLength(encryptionContext) < UINT16_LIMIT;
+      assert Msg.KVPairsLength(encryptionContext) < UINT16_LIMIT;
     }
     var e :- Client.Encrypt(msg, cmm, encryptionContext);
 
