test/SDK/MessageHeader.dfy
@@ -1,0 +1,138 @@
+include "../../src/SDK/AlgorithmSuite.dfy"
+include "../../src/StandardLibrary/StandardLibrary.dfy"
+include "../../src/SDK/Materials.dfy"
+include "../../src/Util/UTF8.dfy"
+include "../../src/SDK/MessageHeader.dfy"
+include "../Util/TestUtils.dfy"
+
+module TestMessageHeader {
+  import AlgorithmSuite
+  import opened StandardLibrary
+  import opened UInt = StandardLibrary.UInt
+  import Materials
+  import UTF8
+  import MessageHeader
+  import TestUtils
+
+  method {:test} TestValidKVPair() returns (r: Result<()>) {
+    var keyA, valA := UTF8.Encode("keyA").value, UTF8.Encode("valA").value;
+    var kvPair := (keyA, valA);
+    r := Require(MessageHeader.ValidKVPair(kvPair));
+  }
+
+  method {:test} TestValidKVPairTooLong() returns (r: Result<()>) {
+    var keyA := UTF8.Encode("keyA").value;
+    var invalidVal := seq(0x1_0000, _ => 0);
+    TestUtils.AssumeLongSeqIsValidUTF8(invalidVal);
+    var kvPair := (keyA, invalidVal);
+    r := Require(!MessageHeader.ValidKVPair(kvPair));
+  }
+
+  method {:test} TestKVPairEntriesLength() returns (r: Result<()>) {
+    var keyA, valA := UTF8.Encode("keyA").value, UTF8.Encode("valA").value;
+    var kvPairs := [(keyA, valA)];
+    var len := MessageHeader.KVPairEntriesLength(kvPairs, 0, |kvPairs|);
+
+    r := RequireEqual(len, 2 + |keyA| + 2 + |valA|);
+  }
+
+  method {:test} TestKVPairsLength() returns (r: Result<()>) {
+    var keyA, valA := UTF8.Encode("keyA").value, UTF8.Encode("valA").value;
+    var kvPairs := [(keyA, valA)];
+    var len := MessageHeader.KVPairsLength(kvPairs);
+
+    r := RequireEqual(len, 2 + 2 + |keyA| + 2 + |valA|);
+  }
+
+  method {:test} TestValidAAD() returns (r: Result<()>) {
+    var keyA, valA := UTF8.Encode("keyA").value, UTF8.Encode("valA").value;
+    var kvPairs := [(keyA, valA)];
+    r := Require(MessageHeader.ValidAAD(kvPairs));
+  }
+
+  method {:test} TestValidAADInvalidPairs() returns (r: Result<()>) {
+    var keyA := UTF8.Encode("keyA").value;
+    var invalidVal := seq(0x1_0000, _ => 0);
+    TestUtils.AssumeLongSeqIsValidUTF8(invalidVal);
+    var kvPairs := [(keyA, invalidVal)];
+    r := Require(!MessageHeader.ValidAAD(kvPairs));
+  }
+
+  // TODO test for true if EC is just under serialization size limit of 0x1_0000
+
+  // TODO test for false if EC exceeds serialization size limit of 0x1_0000
+  
+  method {:test} TestValidKVPairs() returns (r: Result<()>) {
+    var keyA, valA := UTF8.Encode("keyA").value, UTF8.Encode("valA").value;
+    var kvPairs := [(keyA, valA)];
+    r := Require(MessageHeader.ValidKVPairs(kvPairs));
+  }
+
+  method {:test} TestValidKVPairsInvalidPair() returns (r: Result<()>) {
+    var keyA := UTF8.Encode("keyA").value;
+    var invalidVal := seq(0x1_0000, _ => 0);
+    TestUtils.AssumeLongSeqIsValidUTF8(invalidVal);
+    var kvPairs := [(keyA, invalidVal)];
+    r := Require(!MessageHeader.ValidKVPairs(kvPairs));
+  }
+
+  method {:test} TestValidKVPairsUnsorted() returns (r: Result<()>) {
+    var keyA, valA := UTF8.Encode("keyA").value, UTF8.Encode("valA").value;
+    var keyB, valB := UTF8.Encode("keyB").value, UTF8.Encode("valB").value;
+    var kvPairs := [(keyB, valB), (keyA, valA)];
+    r := Require(!MessageHeader.ValidKVPairs(kvPairs));
+  }
+
+  method {:test} TestSortedKVPairs() returns (r: Result<()>) {
+    var keyA, valA := UTF8.Encode("keyA").value, UTF8.Encode("valA").value;
+    var keyB, valB := UTF8.Encode("keyB").value, UTF8.Encode("valB").value;
+    var kvPairs := [(keyA, valA), (keyB, valB)];
+    r := Require(MessageHeader.SortedKVPairs(kvPairs));
+  }
+
+  method {:test} TestSortedKVPairsHasDuplicate() returns (r: Result<()>) {
+    var keyA, valA := UTF8.Encode("keyA").value, UTF8.Encode("valA").value;
+    var kvPairs := [(keyA, valA), (keyA, valA)];
+    r := Require(MessageHeader.SortedKVPairs(kvPairs));
+  }
+
+  method {:test} TestSortedKVPairsEmpty() returns (r: Result<()>) {
+    r := Require(MessageHeader.SortedKVPairs([]));
+  }
+
+  method {:test} TestSortedKVPairsUnsorted() returns (r: Result<()>) {
+    var keyA, valA := UTF8.Encode("keyA").value, UTF8.Encode("valA").value;
+    var keyB, valB := UTF8.Encode("keyB").value, UTF8.Encode("valB").value;
+    var kvPairs := [(keyB, valB), (keyA, valA)];
+    r := Require(!MessageHeader.ValidKVPairs(kvPairs));
+  }
+
+  method {:test} TestKVPairsToSeq() returns (r: Result<()>) {
+    var keyA, valA := UTF8.Encode("keyA").value, UTF8.Encode("valA").value;
+    var kvPairs := [(keyA, valA)];
+    reveal MessageHeader.ValidKVPairs();
+    var expectedBytes := [0, 1, 0, 4, 107, 101, 121, 65, 0, 4, 118, 97, 108, 65];
+    r := RequireEqual(MessageHeader.KVPairsToSeq(kvPairs), expectedBytes);
+  }
+
+  // TODO: test KVPairsToSeq up to serialization size limit (2^16)
+
+  method {:test} TestKVPairEntriesToSeq() returns (r: Result<()>) {
+    var keyA, valA := UTF8.Encode("keyA").value, UTF8.Encode("valA").value;
+    var keyB, valB := UTF8.Encode("keyB").value, UTF8.Encode("valB").value;
+    var kvPairs := [(keyA, valA), (keyB, valB)];
+    var expectedBytes := [0, 4, 107, 101, 121, 65, 0, 4, 118, 97, 108, 65, 0, 4, 107, 101, 121, 66, 0, 4, 118, 97, 108, 66];
+    r := RequireEqual(MessageHeader.KVPairEntriesToSeq(kvPairs, 0, |kvPairs|), expectedBytes);
+  }
+
+  // TODO: test KVPairEntriesToSeq up to serialization size limit (2^16 - 2)
+
+  method {:test} TestKVPairToSeq() returns (r: Result<()>) {
+    var keyA, valA := UTF8.Encode("keyA").value, UTF8.Encode("valA").value;
+    var kvPair := (keyA, valA);
+    var expectedBytes := [0, 4, 107, 101, 121, 65, 0, 4, 118, 97, 108, 65];
+    r := RequireEqual(MessageHeader.KVPairToSeq(kvPair), expectedBytes);
+  }
+
+  // TODO: test KVPairEntriesToSeq up to serialization size limit (2^16 - 4)
+}
